added some docstrings and shortend proofs

Cslib/Languages/LambdaCalculus/LocallyNameless/Untyped/MultiSubst.lean
@@ -5,8 +5,6 @@ public import Cslib.Foundations.Data.HasFresh
 public import Cslib.Foundations.Syntax.HasSubstitution
 public import Cslib.Languages.LambdaCalculus.LocallyNameless.Stlc.Basic
 public import Cslib.Languages.LambdaCalculus.LocallyNameless.Untyped.FullBeta
-public import Cslib.Languages.LambdaCalculus.LocallyNameless.Untyped.StrongNorm
-
 
 @[expose] public section
 
@@ -19,111 +17,84 @@ namespace LambdaCalculus.LocallyNameless.Untyped.Term
 
 variable {Var : Type u} {Base : Type v} [DecidableEq Var] [HasFresh Var]
 
-
+/-- An environment in context of multi substition is a list of pairs of
+    variable targets and terms to be substituted for that target -/
 abbrev Environment (Var : Type u) := Context Var (Term Var)
 
+/-- multi-substitution substitutes all target variables
+    in an environment by their corresponding terms -/
 def multiSubst (σ : Environment Var) (M : Term Var) : Term Var :=
   match σ with
   | [] => M
   | ⟨ i, sub ⟩ :: σ' => (multiSubst σ' M) [ i := sub ]
 
+/-- the free variables of an environment are the union of
+    the free variables of all terms in the environment.
+    The target variables are not necessarily included -/
 def Environment.fv (Ns : Environment Var) : Finset Var :=
   match Ns with
   | [] => {}
   | ⟨ _, sub ⟩ :: Ns' => sub.fv ∪ fv Ns'
 
+/-- an environment is locally closed if all terms in the environment are locally closed -/
+@[simp, grind .]
+def env_LC (Γ : Environment Var) : Prop := ∀ {x M}, ⟨ x, M ⟩ ∈ Γ → LC M
 
-@[simp]
-def env_LC (Γ : Environment Var) : Prop :=
-  ∀ {x M}, ⟨ x, M ⟩ ∈ Γ → LC M
 
+omit [DecidableEq Var] [HasFresh Var] in
+/-- adding a locally closed term to an environment preserves local closure -/
 lemma env_LC_cons {Γ : Environment Var} {x : Var} {sub : Term Var}
-  (lc_sub : LC sub)
-  (lc_Γ : env_LC Γ)
+  (lc_sub : LC sub) (lc_Γ : env_LC Γ)
   : env_LC (⟨ x, sub ⟩ :: Γ) := by
   intro y M h_mem
   cases h_mem <;> aesop
 
-
-
+/-- multi-substitution of a fresh variable does nothing -/
 def multiSubst_fvar_fresh (Ns : Environment Var) :
-  ∀ x ∉ Ns.dom, multiSubst Ns (Term.fvar x) = Term.fvar x := by
-  induction Ns <;> intro x h_fresh
-  · case nil =>
-      simp [multiSubst]
-  · case cons N Ns ih =>
-      simp only [multiSubst]
-      simp only [Context.dom] at h_fresh
-      rw[ih]
-      · rw[subst_fvar]
-        by_cases h : N.1 = x <;> simp_all
-      · simp_all
+    ∀ x ∉ Ns.dom, multiSubst Ns (Term.fvar x) = Term.fvar x := by
+  induction Ns
+  · case nil => simp [multiSubst]
+  · case cons N Ns ih => cases N ; simp_all ; grind[multiSubst]
 
+omit [HasFresh Var] in
 lemma multiSubst_preserves_not_fvar {x : Var}
   (M : Term Var)
   (Ns : Environment Var)
   (nmem : x ∉ M.fv ∪ Ns.fv) :
-  x ∉ (multiSubst Ns M).fv := by
-  induction Ns
-  · case nil =>
-      rw[multiSubst]
-      simp_all
-  · case cons N Ns ih =>
-      rw[multiSubst]
-      apply subst_preserve_not_fvar
-      rw[Environment.fv] at nmem
-      simp_all
+    x ∉ (multiSubst Ns M).fv := by
+  induction Ns <;> grind[multiSubst, subst_preserve_not_fvar, Environment.fv]
 
+/-- multi-substitution propagates recursively through an application -/
 def multiSubst_app (M N : Term Var) (Ps : Environment Var) :
-        multiSubst Ps (Term.app M N) = Term.app (multiSubst Ps M) (multiSubst Ps N) := by
-  induction Ps
-  · rfl
-  · case cons N Ns ih => rw[multiSubst, multiSubst, ih]; rfl
+      multiSubst Ps (Term.app M N) = Term.app (multiSubst Ps M) (multiSubst Ps N) := by
+  induction Ps <;> grind[multiSubst]
 
+/-- multi-substitution propagates recursively through an abstraction -/
 def multiSubst_abs (M : Term Var) (Ns : Environment Var) :
-    multiSubst Ns (Term.abs M) =
-    Term.abs (multiSubst Ns M) := by
-  induction Ns
-  · rfl
-  · case cons N Ns ih => rw[multiSubst, ih]; rfl
+      multiSubst Ns (Term.abs M) = Term.abs (multiSubst Ns M) := by
+  induction Ns <;> grind[multiSubst]
 
+omit [HasFresh Var] in
 lemma open'_fvar_subst (M N : Term Var) (x : Var) (H : x ∉ Term.fv M) :
-  (i : Nat) → (M ⟦ i ↝ Term.fvar x ⟧) [x := N] = M ⟦ i ↝ N ⟧ := by
-  induction M <;> intro i
-  · case bvar j =>
-      rw[Term.openRec_bvar, Term.openRec_bvar]
-      by_cases h : i = j <;> simp[h, Term.subst_fvar, Term.subst_bvar]
-  · case fvar y =>
-      rw[Term.openRec_fvar, Term.openRec_fvar]
-      simp only [Term.fv, Finset.mem_singleton] at H
-      simp only [subst_fvar, ite_eq_right_iff]
-      intro H
-      contradiction
-  · case abs M ih =>
-      rw[Term.openRec_abs, Term.openRec_abs]
-      rw[Term.subst_abs]
-      rw[ih H]
-  · case app l r ih_l ih_r =>
-      rw[Term.openRec_app, Term.openRec_app]
-      rw[Term.subst_app]
-      simp only [Term.fv, Finset.mem_union, not_or] at H
-      rw[ih_l H.1]
-      rw[ih_r H.2]
+    (i : Nat) → (M ⟦ i ↝ Term.fvar x ⟧) [x := N] = M ⟦ i ↝ N ⟧ := by
+  induction M <;> grind
 
-lemma multiSubst_open_var (M : Term Var) (Ns : Environment Var) (x : Var) :
-  x ∉ Ns.dom →
-  env_LC Ns →
-  (multiSubst Ns (M ^ (Term.fvar x))) =
-  (multiSubst Ns M) ^ (Term.fvar x) := by
-  intro h_ndom h_lc
+lemma multiSubst_open_var (M : Term Var) (Ns : Environment Var) (x : Var)
+  (h_ndom : x ∉ Ns.dom)
+  (h_lc : env_LC Ns) :
+    (multiSubst Ns (M ^ (Term.fvar x))) = (multiSubst Ns M) ^ (Term.fvar x) := by
   induction Ns with
   | nil => rfl
   | cons N Ns ih =>
     rw[multiSubst, multiSubst]
     rw[ih]
-    · rw[subst_open_var] <;> aesop
+    · rw[subst_open_var]
+      · cases N
+        simp_all
+        grind
+      · grind
     · simp_all
-    aesop
+    grind
 
 end LambdaCalculus.LocallyNameless.Untyped.Term
 
